---
id: basic_algebra
title: Basic Algebra
sidebar_label: Basic Algebra
---

## Identities

- $x^n - 1 = (x - 1)(x^{n - 1} + x^{n - 2} + ... + x + 1)$ for $n \geq 1$.
- $x^n - y^n = (x - y)(x^{n - 1} + x^{n - 2}y + ... + xy^{n - 2} + y^{n - 1})$ for $n \geq 1$.
- In above equality for odd $n$, replacing $y$ with $-y$ gives, $x^n + y^n = (x + y)(x^{n - 1} - x^{n - 2}y + ... - xy^{n - 2} + y^{n - 1})$
- $(1 + x)^n = 1 + nx + \frac{n(n - 1)}{2!}x^2 + \frac{n(n - 1)(n - 2)}{3!}x^3 + \dots$ is valid only for $|x| < 1$
- $(a + b + c)^2 = a^2 + b^2 + c^2 + 2ab + 2bc + 2ca$

  Thus $(D^2 + D + 1)^2 = D^4 + 3D^2 + 2D^3 + 2D + 1$
